Veir/IR/InBounds.lean
@@ -165,53 +165,59 @@ theorem OperationPtr.setBlockOperands_OpOperandPtr_InBounds_mono_ne {opOperand :
 
 @[grind =]
 theorem OperationPtr.setProperties_genericPtr_mono (ptr : GenericPtr)  :
-    ptr.InBounds (setProperties op ctx newProperties h) ↔ ptr.InBounds ctx := by
+    ptr.InBounds (setProperties op ctx h newProperties) ↔ ptr.InBounds ctx := by
   grind
 
 @[grind .]
 theorem OpResultPtr.allocEmpty_no_results {opResult : OpResultPtr}
-    (heq : OperationPtr.allocEmpty ctx ty = some (ctx', op')) :
+    (heq : OperationPtr.allocEmpty ctx ty properties = some (ctx', op')) :
     opResult.op = op' → ¬ opResult.InBounds ctx' := by
   grind
 
 @[grind .]
 theorem OpOperandPtr.allocEmpty_no_operands {opOperand : OpOperandPtr}
-    (heq : OperationPtr.allocEmpty ctx ty = some (ctx', op')) :
+    (heq : OperationPtr.allocEmpty ctx ty properties = some (ctx', op')) :
     opOperand.op = op' → ¬ opOperand.InBounds ctx' := by
   grind
 
 @[grind .]
 theorem BlockOperandPtr.allocEmpty_no_operands {blockOperand : BlockOperandPtr}
-    (heq : OperationPtr.allocEmpty ctx ty = some (ctx', op')) :
+    (heq : OperationPtr.allocEmpty ctx ty properties = some (ctx', op')) :
     blockOperand.op = op' → ¬ blockOperand.InBounds ctx' := by
   grind
 
 @[grind .]
-theorem OperationPtr.allocEmpty_genericPtr_iff (ptr : GenericPtr) (heq : allocEmpty ctx type = some (ctx', ptr')) :
+theorem OperationPtr.allocEmpty_genericPtr_iff (ptr : GenericPtr)
+    (heq : allocEmpty ctx type properties = some (ctx', ptr')) :
     ptr.InBounds ctx' ↔ (ptr.InBounds ctx ∨ ptr = .operation ⟨ctx.nextID⟩) := by
   grind
 
 -- TODO: make this the main statement?
-theorem OperationPtr.allocEmpty_genericPtr_iff' (ptr : GenericPtr) (heq : allocEmpty ctx type = some (ctx', ptr')) :
+theorem OperationPtr.allocEmpty_genericPtr_iff' (ptr : GenericPtr)
+    (heq : allocEmpty ctx type properties = some (ctx', ptr')) :
     ptr.InBounds ctx' ↔ (ptr.InBounds ctx ∨ ptr = .operation ptr') := by
   grind
 
-theorem OperationPtr.allocEmpty_operationPtr_iff (ptr : OperationPtr) (heq : allocEmpty ctx type = some (ctx', ptr')) :
+theorem OperationPtr.allocEmpty_operationPtr_iff (ptr : OperationPtr)
+    (heq : allocEmpty ctx type properties = some (ctx', ptr')) :
     ptr.InBounds ctx' ↔ (ptr.InBounds ctx ∨ ptr =  ptr') := by
   grind
 
 @[grind . ]
-theorem OperationPtr.allocEmpty_genericPtr_mono (ptr : GenericPtr) (heq : allocEmpty ctx type = some (ctx', ptr')) :
+theorem OperationPtr.allocEmpty_genericPtr_mono (ptr : GenericPtr)
+    (heq : allocEmpty ctx type properties = some (ctx', ptr')) :
     ptr.InBounds ctx → ptr.InBounds ctx' := by
   grind
 
 @[grind .]
-theorem OperationPtr.allocEmpty_not_inBounds (heq : allocEmpty ctx type = some (ctx', ptr')) :
+theorem OperationPtr.allocEmpty_not_inBounds
+    (heq : allocEmpty ctx type properties = some (ctx', ptr')) :
     ¬ ptr'.InBounds ctx := by
   grind
 
 @[grind .]
-theorem OperationPtr.allocEmpty_newBlock_inBounds (heq : allocEmpty ctx type = some (ctx', ptr)) :
+theorem OperationPtr.allocEmpty_newBlock_inBounds
+    (heq : allocEmpty ctx type properties = some (ctx', ptr)) :
     ptr.InBounds ctx' := by
   grind
 
